examples/dsl/FStar.Meta.Tc.Builtins.fsti
@@ -3,4 +3,6 @@ module FStar.Meta.Tc.Builtins
 open FStar.Reflection.Types
 open FStar.Meta.Tc.Effect
 
-val tc_term (en:env) (t:term) : MetaTcT term
+val valid_prop (en:env) (t:typ) : Type0
+
+val check_prop_validity (en:env) (t:typ) : MetaTcT (valid_prop en t)
